Fix semantics and soundness. Some work in proof theory pattern.

PropositionalLogic/Semantics/Trivial.v
@@ -17,45 +17,122 @@ Definition orp {model: Type} (X: Ensemble model) (Y: Ensemble model): Ensemble m
 
 Definition falsep {model: Type}: Ensemble model := fun m => False.
 
+Definition truep {model: Type}: Ensemble model := fun m => True.
+
+Definition iffp {model: Type} (X: Ensemble model) (Y: Ensemble model): Ensemble model :=
+  fun m => X m <-> Y m.
+
+Definition negp {model: Type} (X: Ensemble model): Ensemble model :=
+  fun m => ~ X m.
+
 End Semantics.
 
-Class TrivialPropositionalSemantics (L: Language) {minL: MinimumLanguage L} {pL: PropositionalLanguage L} (MD: Model) (SM: Semantics L MD): Type := {
+Class AndSemantics
+      (L: Language)
+      {andpL: AndLanguage L}
+      (MD: Model)
+      (SM: Semantics L MD): Type := {
   denote_andp: forall x y, Same_set _ (denotation (x && y)) (Semantics.andp (denotation x) (denotation y));
+}.
+
+Class OrSemantics
+      (L: Language)
+      {orpL: OrLanguage L}
+      (MD: Model)
+      (SM: Semantics L MD): Type := {
   denote_orp: forall x y, Same_set _ (denotation (x || y)) (Semantics.orp (denotation x) (denotation y));
+}.
+
+Class FalseSemantics
+      (L: Language)
+      {falsepL: FalseLanguage L}
+      (MD: Model)
+      (SM: Semantics L MD): Type := {
   denote_falsep: Same_set _ (denotation FF) Semantics.falsep
+}.
+
+Class TrueSemantics
+      (L: Language)
+      {truepL: TrueLanguage L}
+      (MD: Model)
+      (SM: Semantics L MD): Type := {
+  denote_truep: Same_set _ (denotation TT) Semantics.truep
+}.
+
+Class IffSemantics
+      (L: Language)
+      {iffpL: IffLanguage L}
+      (MD: Model)
+      (SM: Semantics L MD): Type := {
+  denote_iffp: forall x y, Same_set _ (denotation (x <--> y)) (Semantics.iffp (denotation x) (denotation y));
+}.
+
+Class NegSemantics
+      (L: Language)
+      {negpL: NegLanguage L}
+      (MD: Model)
+      (SM: Semantics L MD): Type := {
+  denote_negp: forall x, Same_set _ (denotation (~~ x)) (Semantics.negp (denotation x));
 }.
 
 Section Trivial.
 
 Context {L: Language}
-        {minL: MinimumLanguage L}
-        {pL: PropositionalLanguage L}
         {MD: Model}
-        {SM: Semantics L MD}
-        {tpSM: TrivialPropositionalSemantics L MD SM}.
+        {SM: Semantics L MD}.
 
-Lemma sat_andp: forall m x y, m |= x && y <-> (m |= x /\ m |= y).
+Lemma sat_andp {andpL: AndLanguage L} {andpSM: AndSemantics L MD SM}:
+  forall m x y, m |= x && y <-> (m |= x /\ m |= y).
 Proof.
   intros; simpl.
   unfold satisfies.
   destruct (denote_andp x y).
-  split; auto; [apply H | apply H0].
+  split; [apply H | apply H0].
 Qed.
 
-Lemma sat_orp: forall m x y, m |= x || y <-> (m |= x \/ m |= y).
+Lemma sat_orp {orpL: OrLanguage L} {orpSM: OrSemantics L MD SM}:
+  forall m x y, m |= x || y <-> (m |= x \/ m |= y).
 Proof.
   intros; simpl.
   unfold satisfies.
   destruct (denote_orp x y).
-  split; auto; [apply H | apply H0].
+  split; [apply H | apply H0].
 Qed.
 
-Lemma sat_falsep: forall m, m |= FF <-> False.
+Lemma sat_falsep {falsepL: FalseLanguage L} {falsepSM: FalseSemantics L MD SM}:
+  forall m, m |= FF <-> False.
 Proof.
   intros; simpl.
   unfold satisfies.
   destruct denote_falsep.
-  split; auto; [apply H | apply H0].
+  split; [apply H | apply H0].
+Qed.
+
+Lemma sat_truep {truepL: TrueLanguage L} {truepSM: TrueSemantics L MD SM}:
+  forall m, m |= TT <-> True.
+Proof.
+  intros; simpl.
+  unfold satisfies.
+  destruct denote_truep.
+  split; [apply H | apply H0].
+Qed.
+
+Lemma sat_iffp {iffpL: IffLanguage L} {iffpSM: IffSemantics L MD SM}:
+  forall m x y, m |= x <--> y <-> (m |= x <-> m |= y).
+Proof.
+  intros; simpl.
+  unfold satisfies.
+  destruct (denote_iffp x y).
+  split; [apply H | apply H0].
+Qed.
+
+Lemma sat_negp {negpL: NegLanguage L} {negpSM: NegSemantics L MD SM}:
+  forall m x, m |= ~~ x  <-> ~ (m |= x).
+Proof.
+  intros; simpl.
+  unfold satisfies.
+  destruct (denote_negp x).
+  split; [apply H | apply H0].
 Qed.
 
 End Trivial.
