PropositionalLogic/ProofTheory/Intuitionistic.v
@@ -591,6 +591,24 @@ Proof.
   auto.
 Qed.
 
+Lemma solve_iffp_elim1: forall x y: expr,
+  |-- x <--> y ->
+  |-- x --> y.
+Proof.
+  intros.
+  pose proof iffp_elim1 x y.
+  eapply modus_ponens; eauto.
+Qed.
+
+Lemma solve_iffp_elim2: forall x y: expr,
+  |-- x <--> y ->
+  |-- y --> x.
+Proof.
+  intros.
+  pose proof iffp_elim2 x y.
+  eapply modus_ponens; eauto.
+Qed.
+
 Lemma solve_impp_elim_left: forall x y: expr,
   |-- y -> |-- x --> y.
 Proof.
@@ -648,10 +666,9 @@ Qed.
 Lemma provable_iffp_refl: forall (x: expr),
   |-- x <--> x.
 Proof.
-  AddSequentCalculus.
   intros.
-  rewrite provable_derivable.
-  apply derivable_iffp_refl.
+  apply solve_iffp_intros;
+  apply provable_impp_refl.
 Qed.
 
 Lemma contrapositivePP: forall (x y: expr),
@@ -800,23 +817,27 @@ Proof.
   apply truep_intros.
 Qed.
 
-Lemma andp_comm: forall (x y: expr),
-  |-- x && y <--> y && x.
+Lemma andp_comm_impp: forall (x y: expr),
+  |-- x && y --> y && x.
 Proof.
+  clear - minAX andpAX.
   AddSequentCalculus.
   intros.
   rewrite provable_derivable.
-  apply deduction_iffp_intros.
-  + apply deduction_andp_intros.
-    - eapply deduction_andp_elim2.
-      apply derivable_assum1.
-    - eapply deduction_andp_elim1.
-      apply derivable_assum1.
-  + apply deduction_andp_intros.
-    - eapply deduction_andp_elim2.
-      apply derivable_assum1.
-    - eapply deduction_andp_elim1.
-      apply derivable_assum1.
+  rewrite <- deduction_theorem.
+  apply deduction_andp_intros.
+  + eapply deduction_andp_elim2.
+    apply derivable_assum1.
+  + eapply deduction_andp_elim1.
+    apply derivable_assum1.
+Qed.
+
+Lemma andp_comm: forall (x y: expr),
+  |-- x && y <--> y && x.
+Proof.
+  intros.
+  apply solve_iffp_intros;
+  apply andp_comm_impp.
 Qed.
 
 Lemma andp_assoc: forall (x y z: expr),
@@ -991,6 +1012,7 @@ Qed.
 Lemma impp_curry: forall (x y z: expr),
   |-- (x --> y --> z) --> (x && y --> z).
 Proof.
+  clear - minAX andpAX.
   AddSequentCalculus.
   intros.
   rewrite provable_derivable.
@@ -1007,6 +1029,7 @@ Qed.
 Lemma impp_uncurry: forall (x y z: expr),
   |-- (x && y --> z) --> (x --> y --> z).
 Proof.
+  clear - minAX andpAX.
   AddSequentCalculus.
   intros.
   rewrite provable_derivable.
@@ -1020,10 +1043,8 @@ Qed.
 Lemma impp_curry_uncurry: forall (x y z: expr),
   |-- (x --> y --> z) <--> (x && y --> z).
 Proof.
-  AddSequentCalculus.
   intros.
-  rewrite provable_derivable.
-  apply deduction_iffp_intros; rewrite deduction_theorem; rewrite <- provable_derivable.
+  apply solve_iffp_intros.
   + apply impp_curry.
   + apply impp_uncurry.
 Qed.
